<?xml version="1.0"?>
<rdf:RDF xmlns:dsv="http://purl.org/iso25964/DataSet/Versioning#" xml:base="http://purl.org/iso25964/DataSet/Versioning" xmlns:dc="http://purl.org/dc/elements/1.1/" xmlns:rdfs="http://www.w3.org/2000/01/rdf-schema#" xmlns:owl="http://www.w3.org/2002/07/owl#" xmlns:xsd="http://www.w3.org/2001/XMLSchema#" xmlns:rdf="http://www.w3.org/1999/02/22-rdf-syntax-ns#" xmlns:skos="http://www.w3.org/2004/02/skos/core#" xmlns:dcterms="http://purl.org/dc/terms/" xmlns:vs="http://www.w3.org/2003/06/sw-vocab-status/ns#" xmlns:foaf="http://xmlns.com/foaf/0.1/">
	<owl:Ontology rdf:about="http://purl.org/iso25964/DataSet/Versioning">
		<rdfs:comment xml:lang="en">Defines a class capturing the version (release or publication of) a dataseet (e.g. a Thesaurus) publication in a SPARQL end-point, an LOD publication or a DCAT dataset publication.

See Version History Proposal specifying:
- a version history set (dsv:VersionHistorySet) with fixed URI for its unique thesaurus version set instance, and
- a version history record instance (dsv:VersionHistoryRecord) with a thesaurus version specific URI corresponds the ISO 25964 VersionHistory.
</rdfs:comment>
		<rdfs:seeAlso rdf:resource="http://www.niso.org/schemas/iso25964/correspondencesSKOS/"/>
		<dcterms:created rdf:datatype="http://www.w3.org/2001/XMLSchema#date">2013-10-04</dcterms:created>
		<dcterms:modified rdf:datatype="http://www.w3.org/2001/XMLSchema#date">2014-07-31</dcterms:modified>
		<dcterms:title xml:lang="en">Dataset Versioning ontology</dcterms:title>
		<dcterms:creator foaf:name="Johan De Smedt"/>
	</owl:Ontology>
	<!-- 
    ///////////////////////////////////////////////////////////////////////////////////////
    //
    // Datatypes
    //
    ///////////////////////////////////////////////////////////////////////////////////////
     -->
	<!-- 
    ///////////////////////////////////////////////////////////////////////////////////////
    //
    // Object Properties
    //
    ///////////////////////////////////////////////////////////////////////////////////////
     -->
	<!-- http://purl.org/iso25964/DataSet/Versioning#currentVersionRecord -->
	<owl:ObjectProperty rdf:about="http://purl.org/iso25964/DataSet/Versioning#currentVersionRecord">
		<rdfs:label xml:lang="en">current version record</rdfs:label>
		<rdfs:comment xml:lang="en">dsv:currentVersionRecord on a version set details the last published version. 
The object of this property is a dsv:VersionHistoryRecord</rdfs:comment>
		<rdfs:isDefinedBy rdf:resource="http://purl.org/iso25964/DataSet/Versioning"/>
		<rdfs:range rdf:resource="http://purl.org/iso25964/DataSet/Versioning#VersionHistoryRecord"/>
		<rdfs:domain rdf:resource="http://purl.org/iso25964/DataSet/Versioning#VersionHistorySet"/>
		<dcterms:modified rdf:datatype="http://www.w3.org/2001/XMLSchema#date">2013-10-04</dcterms:modified>
		<vs:term_status>proposed</vs:term_status>
	</owl:ObjectProperty>
	<!-- http://purl.org/iso25964/DataSet/Versioning#hasVersionRecord -->
	<owl:ObjectProperty rdf:about="http://purl.org/iso25964/DataSet/Versioning#hasVersionRecord">
		<rdfs:label xml:lang="en">has version record</rdfs:label>
		<rdfs:isDefinedBy rdf:resource="http://purl.org/iso25964/DataSet/Versioning"/>
		<rdfs:range rdf:resource="http://purl.org/iso25964/DataSet/Versioning#VersionHistoryRecord"/>
		<dcterms:modified rdf:datatype="http://www.w3.org/2001/XMLSchema#date">2013-10-04</dcterms:modified>
		<vs:term_status>proposed</vs:term_status>
	</owl:ObjectProperty>
	<!-- http://purl.org/iso25964/DataSet/Versioning#hasVersionHistorySet -->
	<owl:ObjectProperty rdf:about="http://purl.org/iso25964/DataSet/Versioning#hasVersionHistorySet">
		<rdfs:label xml:lang="en">has version history set</rdfs:label>
		<rdfs:comment xml:lang="en">Each VersionHistoryRecord identifies its Version History Set with exactly one dsv:hasVersionHistorySet object property. 
The mandatory attribute identifier may be mapped to the Dublin Core property dc:identifier. 
The date attribute is mapped to the Dublin Core property dc:date. 
The versionNote can be mapped to skos:note.</rdfs:comment>
		<rdfs:isDefinedBy rdf:resource="http://purl.org/iso25964/DataSet/Versioning"/>
		<rdfs:domain rdf:resource="http://purl.org/iso25964/DataSet/Versioning#VersionHistoryRecord"/>
		<rdfs:range rdf:resource="http://purl.org/iso25964/DataSet/Versioning#VersionHistorySet"/>
		<dcterms:modified rdf:datatype="http://www.w3.org/2001/XMLSchema#date">2013-10-04</dcterms:modified>
		<vs:term_status>proposed</vs:term_status>
	</owl:ObjectProperty>
	<!-- http://purl.org/iso25964/DataSet/Versioning#isVersionRecordOf -->
	<owl:ObjectProperty rdf:about="http://purl.org/iso25964/DataSet/Versioning#isVersionRecordOf">
		<rdfs:label xml:lang="en">is version record of</rdfs:label>
		<rdfs:comment xml:lang="en">The object of this property references to the data set end points (SPARQL end-point, LOD, data-set, â€¦). 
There can be any number of dsv:isVersionRecordOf (depending on the physical publications made of that data set version).</rdfs:comment>
		<rdfs:isDefinedBy rdf:resource="http://purl.org/iso25964/DataSet/Versioning"/>
		<owl:inverseOf rdf:resource="http://purl.org/iso25964/DataSet/Versioning#hasVersionRecord"/>
		<dcterms:modified rdf:datatype="http://www.w3.org/2001/XMLSchema#date">2013-10-04</dcterms:modified>
		<vs:term_status>proposed</vs:term_status>
	</owl:ObjectProperty>
	<!-- http://purl.org/iso25964/DataSet/Versioning#requiresDatasetOfVersionRecord -->
	<owl:ObjectProperty rdf:about="http://purl.org/iso25964/DataSet/Versioning#requiresDatasetOfVersionRecord">
		<rdfs:label xml:lang="en">requires dataset version</rdfs:label>
		<rdfs:comment xml:lang="en">The dataset version detailed in the subject dataset record requires the.dataset version detailed by the object dataset record.
Typically the subject dataset version refers resources defined by the object dataset version.
This relation is intended to capture dependencies between dataset versions of different datasets.
Example:
- the source dataset is a (a version of a) SKOS ConceptScheme about certification.
- the object dataset is a (version and/or variant of) a national (or cross national) qualification framework
- certifications may get a tagging to identify the qualification level according a specific qualification framework.</rdfs:comment>
		<rdfs:isDefinedBy rdf:resource="http://purl.org/iso25964/DataSet/Versioning"/>
		<rdfs:domain rdf:resource="http://purl.org/iso25964/DataSet/Versioning#VersionHistoryRecord"/>
		<rdfs:range rdf:resource="http://purl.org/iso25964/DataSet/Versioning#VersionHistoryRecord"/>
		<dcterms:modified rdf:datatype="http://www.w3.org/2001/XMLSchema#date">2014-03-04</dcterms:modified>
		<vs:term_status>proposed</vs:term_status>
	</owl:ObjectProperty>
	<owl:ObjectProperty rdf:about="http://purl.org/dc/terms/isVersionOf">
		<rdfs:label xml:lang="en">Is Version Of</rdfs:label>
		<rdfs:comment xml:lang="en">A related resource of which the described resource is a version, edition, or adaptation.

For a dataset, the object value identifies the dsv:VersionHistorySet of the subject dataset.</rdfs:comment>
		<dcterms:description xml:lang="en">Changes in version imply substantive changes in content rather than differences in format.</dcterms:description>
		<rdfs:isDefinedBy rdf:resource="http://purl.org/dc/terms/"/>
		<dcterms:issued rdf:datatype="http://www.w3.org/2001/XMLSchema#date">2000-07-11</dcterms:issued>
		<dcterms:modified rdf:datatype="http://www.w3.org/2001/XMLSchema#date">2014-07-31</dcterms:modified>
	</owl:ObjectProperty>
	<!-- 
    ///////////////////////////////////////////////////////////////////////////////////////
    //
    // Data properties
    //
    ///////////////////////////////////////////////////////////////////////////////////////
     -->
	<!-- 
    ///////////////////////////////////////////////////////////////////////////////////////
    //
    // Classes
    //
    ///////////////////////////////////////////////////////////////////////////////////////
     -->
	<!-- http://purl.org/iso25964/DataSet/Versioning#VersionHistory -->
	<owl:Class rdf:about="http://purl.org/iso25964/DataSet/Versioning#VersionHistoryRecord">
		<rdfs:label xml:lang="en">Version history record</rdfs:label>
		<rdfs:comment xml:lang="en">Each VersionHistoryRecord identifies its Version History Set with exactly one hasVersionHistorySet object property. 
The mandatory attribute identifier may be mapped to the Dublin Core property dc:identifier.
The date attribute is mapped to the Dublin Core property dc:date. 
The versionNote can be mapped to skos:note.</rdfs:comment>
		<rdfs:isDefinedBy rdf:resource="http://purl.org/iso25964/DataSet/Versioning"/>
		<rdfs:subClassOf>
			<owl:Restriction>
				<owl:onProperty rdf:resource="http://purl.org/iso25964/DataSet/Versioning#hasVersionHistorySet"/>
				<owl:onClass rdf:resource="http://purl.org/iso25964/DataSet/Versioning#VersionHistoryRecord"/>
				<owl:qualifiedCardinality rdf:datatype="http://www.w3.org/2001/XMLSchema#nonNegativeInteger">1</owl:qualifiedCardinality>
			</owl:Restriction>
		</rdfs:subClassOf>
		<dcterms:modified rdf:datatype="http://www.w3.org/2001/XMLSchema#date">2013-10-04</dcterms:modified>
		<vs:term_status>proposed</vs:term_status>
	</owl:Class>
	<!-- http://purl.org/iso25964/DataSet/Versioning#VersionHistorySet -->
	<owl:Class rdf:about="http://purl.org/iso25964/DataSet/Versioning#VersionHistorySet">
		<rdfs:label>Version history set</rdfs:label>
		<rdfs:subClassOf>
			<owl:Restriction>
				<owl:onProperty rdf:resource="http://purl.org/iso25964/DataSet/Versioning#currentVersionRecord"/>
				<owl:onClass rdf:resource="http://purl.org/iso25964/DataSet/Versioning#VersionHistoryRecord"/>
				<owl:qualifiedCardinality rdf:datatype="http://www.w3.org/2001/XMLSchema#nonNegativeInteger">1</owl:qualifiedCardinality>
			</owl:Restriction>
		</rdfs:subClassOf>
		<rdfs:comment xml:lang="en">The VersionHistorySet has exactly one dsv:currentVersionRecord object property to the version set detailing the last published version. The object of this property is the version record describing the Data Set which is current.
(not the latest.)</rdfs:comment>
		<rdfs:isDefinedBy rdf:resource="http://purl.org/iso25964/DataSet/Versioning"/>
		<dcterms:modified rdf:datatype="http://www.w3.org/2001/XMLSchema#date">2013-10-04</dcterms:modified>
		<vs:term_status>proposed</vs:term_status>
	</owl:Class>
	<!-- 
    ///////////////////////////////////////////////////////////////////////////////////////
    //
    // Annotations
    //
    ///////////////////////////////////////////////////////////////////////////////////////
     -->
</rdf:RDF>
<!-- Generated by the OWL API (version 3.2.3.1824) http://owlapi.sourceforge.net -->
