<?xml version="1.0"?>
<rdf:RDF xmlns:ds-vers="http://www.niso.org/schemas/iso25964/DataSet/Versioning#" xml:base="http://www.niso.org/schemas/iso25964/DataSet/Versioning" xmlns:dc="http://purl.org/dc/elements/1.1/" xmlns:rdfs="http://www.w3.org/2000/01/rdf-schema#" xmlns:owl="http://www.w3.org/2002/07/owl#" xmlns:xsd="http://www.w3.org/2001/XMLSchema#" xmlns:rdf="http://www.w3.org/1999/02/22-rdf-syntax-ns#" xmlns:skos="http://www.w3.org/2004/02/skos/core#" xmlns:dcterms="http://purl.org/dc/terms/">
	<owl:Ontology rdf:about="http://www.niso.org/schemas/iso25964/DataSet/Versioning">
		<rdfs:comment xml:lang="en">Suggestion to add a new class capturing the version (release or publication of) a Thesaurus publication in a SPARQL end-point, an LOD publication or a dataset publication.

See Version History Proposal proposing:
- a version history set (ds-vers:VersionHistorySet) with fixed URI for its unique thesaurus version set instance, and
- a version history record instance (ds-vers:VersionHistoryRecord) with a thesaurus version specific URI corresponds the ISO 25964 VersionHistory.
</rdfs:comment>
		<rdfs:seeAlso rdf:resource="http://www.niso.org/apps/group_public/download.php/9627/Correspondence%20ISO25964-SKOSXL-MADS-2012-10-21.pdf"/>
	</owl:Ontology>
	<!-- 
    ///////////////////////////////////////////////////////////////////////////////////////
    //
    // Datatypes
    //
    ///////////////////////////////////////////////////////////////////////////////////////
     -->
	<!-- 
    ///////////////////////////////////////////////////////////////////////////////////////
    //
    // Object Properties
    //
    ///////////////////////////////////////////////////////////////////////////////////////
     -->
	<!-- http://www.niso.org/schemas/iso25964/DataSet/Versioning#currentVersionRecord -->
	<owl:ObjectProperty rdf:about="http://www.niso.org/schemas/iso25964/DataSet/Versioning#currentVersionRecord">
		<rdfs:label xml:lang="en">current version record</rdfs:label>
		<rdfs:comment xml:lang="en">ds-vers:currentVersionRecord on a version set details the last published version. 
The object of this property is a ds-vers:VersionHistoryRecord</rdfs:comment>
		<rdfs:isDefinedBy rdf:resource="http://www.niso.org/schemas/iso25964/DataSet/Versioning"/>
		<rdfs:range rdf:resource="http://www.niso.org/schemas/iso25964/DataSet/Versioning#VersionHistoryRecord"/>
		<rdfs:domain rdf:resource="http://www.niso.org/schemas/iso25964/DataSet/Versioning#VersionHistorySet"/>
	</owl:ObjectProperty>
	<!-- http://www.niso.org/schemas/iso25964/DataSet/Versioning#hasVersionRecord -->
	<owl:ObjectProperty rdf:about="http://www.niso.org/schemas/iso25964/DataSet/Versioning#hasVersionRecord">
		<rdfs:label xml:lang="en">has version</rdfs:label>
		<rdfs:isDefinedBy rdf:resource="http://www.niso.org/schemas/iso25964/DataSet/Versioning"/>
		<rdfs:range rdf:resource="http://www.niso.org/schemas/iso25964/DataSet/Versioning#VersionHistoryRecord"/>
	</owl:ObjectProperty>
	<!-- http://www.niso.org/schemas/iso25964/DataSet/Versioning#hasVersionHistorySet -->
	<owl:ObjectProperty rdf:about="http://www.niso.org/schemas/iso25964/DataSet/Versioning#hasVersionHistorySet">
		<rdfs:label xml:lang="en">has version history set</rdfs:label>
		<rdfs:comment xml:lang="en">Each VersionHistoryRecord identifies its Version History Set with exactly one ds-vers:hasVersionHistorySet object property. 
The mandatory attribute identifier may be mapped to the Dublin Core property dc:identifier. 
The date attribute is mapped to the Dublin Core property dc:date. 
The versionNote can be mapped to skos:note.</rdfs:comment>
		<rdfs:isDefinedBy rdf:resource="http://www.niso.org/schemas/iso25964/DataSet/Versioning"/>
		<rdfs:domain rdf:resource="http://www.niso.org/schemas/iso25964/DataSet/Versioning#VersionHistoryRecord"/>
		<rdfs:range rdf:resource="http://www.niso.org/schemas/iso25964/DataSet/Versioning#VersionHistorySet"/>
	</owl:ObjectProperty>
	<!-- http://www.niso.org/schemas/iso25964/DataSet/Versioning#isVersionRecordOf -->
	<owl:ObjectProperty rdf:about="http://www.niso.org/schemas/iso25964/DataSet/Versioning#isVersionRecordOf">
		<rdfs:label xml:lang="en">is version of</rdfs:label>
		<rdfs:comment xml:lang="en">The object of this property references to the data set end points (SPARQL end-point, LOD, data-set, â€¦). 
There can be any number of ds-vers:isVersionRecordOf (depending on the physical publications made of that data set version).</rdfs:comment>
		<rdfs:isDefinedBy rdf:resource="http://www.niso.org/schemas/iso25964/DataSet/Versioning"/>
		<owl:inverseOf rdf:resource="http://www.niso.org/schemas/iso25964/DataSet/Versioning#hasVersionRecord"/>
	</owl:ObjectProperty>
	<!-- 
    ///////////////////////////////////////////////////////////////////////////////////////
    //
    // Data properties
    //
    ///////////////////////////////////////////////////////////////////////////////////////
     -->
	<!-- 
    ///////////////////////////////////////////////////////////////////////////////////////
    //
    // Classes
    //
    ///////////////////////////////////////////////////////////////////////////////////////
     -->
	<!-- http://www.niso.org/schemas/iso25964/DataSet/Versioning#VersionHistory -->
	<owl:Class rdf:about="http://www.niso.org/schemas/iso25964/DataSet/Versioning#VersionHistoryRecord">
		<rdfs:label xml:lang="en">Version history record</rdfs:label>
		<rdfs:comment xml:lang="en">Each VersionHistoryRecord identifies its Version History Set with exactly one hasVersionHistorySet object property. 
The mandatory attribute identifier may be mapped to the Dublin Core property dc:identifier.
The date attribute is mapped to the Dublin Core property dc:date. 
The versionNote can be mapped to skos:note.</rdfs:comment>
		<rdfs:isDefinedBy rdf:resource="http://www.niso.org/schemas/iso25964/DataSet/Versioning"/>
		<rdfs:subClassOf>
			<owl:Restriction>
				<owl:onProperty rdf:resource="http://www.niso.org/schemas/iso25964/DataSet/Versioning#hasVersionHistorySet"/>
				<owl:onClass rdf:resource="http://www.niso.org/schemas/iso25964/DataSet/Versioning#VersionHistoryRecord"/>
				<owl:qualifiedCardinality rdf:datatype="http://www.w3.org/2001/XMLSchema#nonNegativeInteger">1</owl:qualifiedCardinality>
			</owl:Restriction>
		</rdfs:subClassOf>
	</owl:Class>
	<!-- http://www.niso.org/schemas/iso25964/DataSet/Versioning#VersionHistorySet -->
	<owl:Class rdf:about="http://www.niso.org/schemas/iso25964/DataSet/Versioning#VersionHistorySet">
		<rdfs:label>Version history set</rdfs:label>
		<rdfs:subClassOf>
			<owl:Restriction>
				<owl:onProperty rdf:resource="http://www.niso.org/schemas/iso25964/DataSet/Versioning#currentVersionRecord"/>
				<owl:onClass rdf:resource="http://www.niso.org/schemas/iso25964/DataSet/Versioning#VersionHistoryRecord"/>
				<owl:qualifiedCardinality rdf:datatype="http://www.w3.org/2001/XMLSchema#nonNegativeInteger">1</owl:qualifiedCardinality>
			</owl:Restriction>
		</rdfs:subClassOf>
		<rdfs:comment xml:lang="en">The VersionHistorySet has exactly one ds-vers:currentVersionRecord object property to the version set detailing the last published version. The object of this property is the version record describing the Data Set which is current.
(not the latest.)</rdfs:comment>
		<rdfs:isDefinedBy rdf:resource="http://www.niso.org/schemas/iso25964/DataSet/Versioning"/>
	</owl:Class>
	<!-- 
    ///////////////////////////////////////////////////////////////////////////////////////
    //
    // Annotations
    //
    ///////////////////////////////////////////////////////////////////////////////////////
     -->
</rdf:RDF>
<!-- Generated by the OWL API (version 3.2.3.1824) http://owlapi.sourceforge.net -->
